untimed/CaseStudy/AutomatonExample.thy
@@ -21,7 +21,7 @@ fun myTransition :: "(State \<times>(channel \<rightharpoonup> nat event)) \<Rig
 "myTransition _ = (myState, tsynbOneTick c1)"
 
 lift_definition myAutomaton :: "(State, nat event) automaton" is "(myTransition, myState, tsynbOneTick c1, {c2}, {c1})"
-  by simp
+  by (simp add: automaton_well_def)
 
 
 
